save try outs

Scratch.thy
@@ -9,6 +9,44 @@ begin
    'a la = 'a cell ref ref
 
 *)
+find_consts "_ set" name: fold
+find_theorems "Finite_Set.fold _ _ (insert _ _)"
+find_theorems "comp_fun_commute_on" "Finite_Set.fold"
+
+interpretation mf: comp_fun_commute_on UNIV "((*)::_::comm_monoid_mult \<Rightarrow> _)"
+  apply(unfold_locales)
+  by(auto simp: algebra_simps)
+  
+definition fold_assn where
+  "fold_assn assns = Finite_Set.fold (*) emp assns * \<up>(finite assns)"
+
+lemma fold_assn_emp [simp]: "fold_assn {} = emp"
+  unfolding fold_assn_def
+  by simp
+
+lemma fold_assn_false: "false \<in> S \<Longrightarrow> fold_assn S = false"
+  unfolding fold_assn_def
+  apply(cases "finite S")
+  by(auto simp: mf.fold_rec)
+
+lemma fold_assn_emp': "emp \<in> S \<Longrightarrow> fold_assn S = fold_assn (S - {emp})"
+  unfolding fold_assn_def
+  apply(cases "finite S")
+  by(auto simp: mf.fold_rec)
+
+thm  mf.fold_insert_remove
+
+lemma fold_assn_cons [simp]: "fold_assn (insert x xs) = x * fold_assn (xs - {x})"
+  unfolding fold_assn_def
+  apply(cases "finite xs")
+  by(simp_all add: mf.fold_insert_remove)
+
+lemma fold_assn_in: "x \<in> xs \<Longrightarrow> fold_assn xs = x * fold_assn (xs - {x})"
+  by (metis fold_assn_cons insert_absorb)
+
+(*lemma fold_assn_app: "fold_assn (xs \<union> ys) = fold_assn xs * fold_assn ys"
+  apply(induction xs)
+  by(auto simp: algebra_simps)*)
 
 datatype 'a::"countable" cell = Array "'a array" | Upd nat "'a" "'a cell ref"
 
@@ -19,23 +57,96 @@ instance cell :: (heap) heap
 
 type_synonym 'a la = "'a cell ref"
 
+datatype 'a::"countable" cell' = Array' "'a list" | Upd' nat "'a" "'a cell ref"
 
-datatype 'a la_node = LA_node nat 'a "'a la_node list" "'a cell ref"
-datatype 'a la_tree = LA_tree "'a list" "'a la_node list" "'a cell ref"
+fun cell_assn where
+  "cell_assn (Array' xs) (Array a) = a \<mapsto>\<^sub>a xs"
+| "cell_assn (Upd' i' val' p') (Upd i val p) = \<up>(i = i' \<and> val = val' \<and> p = p')"
+| "cell_assn _ _ = false"
 
-definition fold_assn where
-  "fold_assn assns = fold (*) assns emp"
+definition master_assn :: "('a::heap cell' \<times> 'a cell ref) set \<Rightarrow> assn" where
+  "master_assn C = fold_assn ((\<lambda>(c', p). \<exists>\<^sub>A c. p \<mapsto>\<^sub>r c * cell_assn c' c) ` C)"
 
-fun la_node_assn where
-   "la_node_assn prev (LA_node i a succs p) = (p \<mapsto>\<^sub>r Upd i a prev) * (fold_assn (map (la_node_assn p) succs))"
+find_theorems "_ ` (_ - _)"
+find_theorems "(\<exists>\<^sub>A _. _) = (\<exists>\<^sub>A _. _)"
+find_consts name:precise
 
-fun la_tree_assn where
-  "la_tree_assn (LA_tree vals succs p) = (\<exists>\<^sub>A ap. (p \<mapsto>\<^sub>r Array ap) * (ap  \<mapsto>\<^sub>a vals) * (fold_assn (map (la_node_assn p) succs)))"
+(* 
+lemma fold_assn_in: "x \<in> xs \<Longrightarrow> fold_assn xs = x * fold_assn (xs - {x})"
+  by (metis fold_assn_cons insert_absorb)
+*)
+
+lemma sth: "a \<noteq> false \<Longrightarrow> true * a \<noteq> false"
+  using ent_false ent_iffI ent_refl_true star_aci(2)
+  by (metis ent_false ent_iffI ent_refl_true star_aci(2))
+
+
+lemma testst: "\<lbrakk>a \<mapsto>\<^sub>a xs = true; a \<mapsto>\<^sub>a ys = true\<rbrakk> \<Longrightarrow> xs = ys"
+  by (metis assn_basic_inequalities(5) merge_true_star snga_same_false)
+
+lemma image_iff_2: "z \<notin> f ` A \<longleftrightarrow> \<not>(\<exists>x\<in>A. z = f x)"
+  by blast
+
+lemma open_master_assn: "(c', p) \<in> C \<Longrightarrow> master_assn C = (\<exists>\<^sub>A c. p \<mapsto>\<^sub>r c * cell_assn c' c) * master_assn (C - {(c', p)})"
+  unfolding master_assn_def
+proof(induction "(\<exists>\<^sub>Ac. p \<mapsto>\<^sub>r c * cell_assn c' c) = false")
+  case True
+  then have "false \<in> ((\<lambda>a. case a of (c', p) \<Rightarrow> \<exists>\<^sub>Ac. p \<mapsto>\<^sub>r c * cell_assn c' c) ` C)"
+    using image_iff by fastforce
+
+  with True show ?case 
+    by (simp add: fold_assn_false)
+next
+  case False
+  then have "false \<notin> ((\<lambda>a. case a of (c', p) \<Rightarrow> \<exists>\<^sub>Ac. p \<mapsto>\<^sub>r c * cell_assn c' c) ` C)"
+    sorry
+
+  with False show ?case
+  apply sep_auto
+  apply(subst fold_assn_in[where x = "\<exists>\<^sub>Ac. p \<mapsto>\<^sub>r c * cell_assn c' c"])
+  apply(auto)[]
+  apply(subst image_set_diff)
+  apply auto
+  apply rule
+    apply auto
+    sorry
+qed
+
+ (* apply sep_auto
+  apply(subst fold_assn_in[where x = "\<exists>\<^sub>Ac. p \<mapsto>\<^sub>r c * cell_assn c' c"])
+  apply(auto)[]
+  apply(subst image_set_diff)
+  apply auto
+  apply rule
+  apply auto
+   sorry*)
 
 no_notation Ref.update ("_ := _" 62)
 notation Ref.update ("_ :=\<^sub>R _" 62)
 
-fun node_to_map :: "'a list \<Rightarrow> 'a la_node \<Rightarrow> ('a cell ref \<rightharpoonup> 'a list)" where
+fun la_rel' where
+  "la_rel' C 0 xs a \<longleftrightarrow> (Array' xs, a) \<in> C"
+| "la_rel' C (Suc n) xs a \<longleftrightarrow> (\<exists>i x a' xs'. (Upd' i x a', a) \<in> C \<and> la_rel' C n xs' a' \<and> xs = xs'[i:=x])"
+  
+definition la_rel where
+  "la_rel C xs a \<equiv> \<exists>n. la_rel' C n xs a"
+
+(*datatype 'a la_node = LA_node nat 'a "'a la_node list" "'a cell ref"
+datatype 'a la_tree = LA_tree "'a list" "'a la_node list" "'a cell ref"
+
+
+
+fun la_node_assn where
+   "la_node_assn prev (LA_node i a succs p) = 
+      (p \<mapsto>\<^sub>r Upd i a prev) * (fold_assn (map (la_node_assn p) succs))"
+
+fun la_tree_assn where
+  "la_tree_assn (LA_tree vals succs p) = 
+     (\<exists>\<^sub>A ap. (p \<mapsto>\<^sub>r Array ap) * (ap  \<mapsto>\<^sub>a vals) * (fold_assn (map (la_node_assn p) succs)))"*)
+
+
+
+(*fun node_to_map :: "'a list \<Rightarrow> 'a la_node \<Rightarrow> ('a cell ref \<rightharpoonup> 'a list)" where
   "node_to_map vals (LA_node i a succs p) = (
     let vals' = vals[i:= a] 
     in [p \<mapsto> vals'] ++ fold (++) (map (node_to_map vals') succs) Map.empty
@@ -53,7 +164,7 @@ fun refs_node where
 definition invar_node :: "'a la_node \<Rightarrow> bool" where
   "invar_node node = distinct (refs_node node)"
 
-fun tree_to_map' where
+fun tree_to_map' :: "'a la_tree \<Rightarrow> ('a cell ref \<times> 'a list) list" where
   "tree_to_map' (LA_tree vals succs p) = (p, vals) # concat (map (node_to_map' vals) succs)"
 
 fun refs_tree where
@@ -83,34 +194,97 @@ find_theorems "map_of" "distinct"
 lemma "invar_tree t \<Longrightarrow> distinct (map fst (tree_to_map' t))"
   by (simp add: invar_tree_def tree_to_map'_refs)
 
-definition la_rel where
-  "la_rel t xs p \<longleftrightarrow> map_of (tree_to_map' t) p = Some xs"
-
-definition array_to_la where
+definition la_rel :: "'a la_tree \<Rightarrow> 'a list \<Rightarrow> 'a cell ref \<Rightarrow> bool" where
+  "la_rel t xs p \<longleftrightarrow> map_of (tree_to_map' t) p = Some xs"*)
+                               
+definition array_to_la :: "('a::heap) array \<Rightarrow> 'a la Heap" where
   "array_to_la a = do {
     ref (Array a)
   }"
 
-lemma [simp]: "fold_assn [] = emp"
-  unfolding fold_assn_def
-  by auto
-
 find_theorems "_ \<Longrightarrow>\<^sub>A \<exists>\<^sub>A _. _"
 
-lemma array_to_la: "<a \<mapsto>\<^sub>a xs> array_to_la a <\<lambda>r. \<exists>\<^sub>At. la_tree_assn t * \<up>(la_rel t xs r)>"
-  unfolding array_to_la_def 
+lemma array_to_la: "<a \<mapsto>\<^sub>a xs> array_to_la a <\<lambda>r. \<exists>\<^sub>At. master_assn t * \<up>(la_rel t xs r)>"
+  unfolding array_to_la_def master_assn_def la_rel_def
   apply vcg
   subgoal for r
-    apply(rule ent_ex_postI[where x = "LA_tree xs [] r"])
-    by(sep_auto simp: la_rel_def)
-  .
+    apply(rule ent_ex_postI[where x = "{(Array' xs, r)}"])
+    by(sep_auto simp: exI[where x = "0"] ent_ex_postI[where x = "cell.Array a"])
+  done
 
-partial_function (heap) foo :: "nat \<Rightarrow> nat Heap"  where
-  "foo n = do { 
-      r \<leftarrow> foo (n);
-      return (r + 1)
+partial_function (heap) lookup :: "('a::heap) la  \<Rightarrow> nat \<Rightarrow> 'a Heap" where
+  "lookup la n = do {
+      cell \<leftarrow> !la;
+      case cell of
+        Array array   \<Rightarrow> Array.nth array n
+      | Upd m value r \<Rightarrow> if n = m 
+                         then return value
+                         else lookup r n
   }"
+declare lookup.simps[code]
 
+
+find_theorems "(=)" "(\<Longrightarrow>\<^sub>A)"
+
+lemma [simp]:"cell_assn (Array' xs) c = (\<exists>\<^sub>Aa. \<up>(c = Array a) * a \<mapsto>\<^sub>a xs)"
+  apply(cases c)
+   apply(auto)
+  apply (rule ent_iffI)
+  by sep_auto+
+
+lemma [simp]:"cell_assn (Upd' i x p) c = \<up>(c = Upd i x p)"
+  apply(cases c)
+  by auto
+
+lemma close_master_assn_upd: "a \<mapsto>\<^sub>r Upd i x a' * master_assn (t - {(Upd' i x a', a)}) \<Longrightarrow>\<^sub>A master_assn t"
+  unfolding master_assn_def
+  using fold_assn_in
+  apply(sep_auto simp: )
+  sorry
+
+lemma lookup: "<master_assn t * \<up>(la_rel' t n xs a \<and> i < length xs)> lookup a i <\<lambda>r. master_assn t * \<up>(r = xs!i)>\<^sub>t"
+proof(induction n arbitrary: xs a)
+  case 0
+  then show ?case
+    apply(sep_auto)
+    apply(subst lookup.simps)
+    apply(subst open_master_assn, assumption)
+    apply sep_auto
+    
+     sorry
+next
+  case (Suc n)
+  show ?case
+    apply(sep_auto)
+    apply(subst lookup.simps)
+    apply(subst open_master_assn, assumption)
+    apply(sep_auto)
+     apply (rule ent_frame_fwd[OF close_master_assn_upd], frame_inference)
+    apply sep_auto
+    apply(rule cons_pre_rule[OF close_master_assn_upd])
+    apply (rule cons_post_rule)
+     thm fi_rule
+      apply (rule fi_rule[OF Suc.IH])
+      apply sep_auto
+     apply sep_auto
+     done
+qed
+
+partial_function (heap) update :: "('a::heap) la \<Rightarrow> nat \<Rightarrow> 'a::heap \<Rightarrow> 'a la Heap" where
+  "update la n v = do {
+      old_v \<leftarrow> lookup la n;
+      cell \<leftarrow> !la;
+      new_la \<leftarrow> case cell of       
+         Array array \<Rightarrow> Array.upd n v array \<bind> array_to_la
+       | Upd m w la' \<Rightarrow> 
+            do {
+                tmp \<leftarrow> update la' n v;
+                ref (Upd m w tmp)
+            };
+      la :=\<^sub>R Upd n old_v new_la;
+      return new_la
+  }"
+declare update.simps[code]
 
 definition array_to_la' where
   "array_to_la' n x = do {
@@ -120,8 +294,10 @@ definition array_to_la' where
   }"
 
 definition test where "test = do {
-  r \<leftarrow> array_to_la' 2 (5::nat);
-  return r
+  r \<leftarrow> array_to_la' 3 (5::nat);
+  y \<leftarrow> update r 1 (6::nat);
+  x \<leftarrow> lookup y 2;
+  return x
 }"
 
 ML_val \<open>@{code test} ()\<close>
